08ByteCode/ByteCode.thy
@@ -49,7 +49,7 @@ inductive eval\<^sub>b :: "code\<^sub>b list \<Rightarrow> state\<^sub>b \<Right
 | ev\<^sub>b_apply [simp]: "lookup \<C> p = Some Apply\<^sub>b \<Longrightarrow> 
     \<C> \<tturnstile> S\<^sub>b (v # Lam\<^sub>b \<Delta>' p' n # \<V>) ((\<Delta>, Suc p) # s) \<leadsto>\<^sub>b S\<^sub>b \<V> (([v] # \<Delta>', p') # (\<Delta>, p) # s)"
 | ev\<^sub>b_pushenv [simp]: "lookup \<C> p = Some PushEnv\<^sub>b \<Longrightarrow> 
-    \<C> \<tturnstile> S\<^sub>b (v # \<V>) ((\<Delta>, Suc p) # s) \<leadsto>\<^sub>b S\<^sub>b \<V> ((cons_fst v \<Delta>, p) # s)"
+    \<C> \<tturnstile> S\<^sub>b (v # \<V>) ((\<Delta>, Suc p) # s) \<leadsto>\<^sub>b S\<^sub>b \<V> ((snoc_fst v \<Delta>, p) # s)"
 | ev\<^sub>b_return [simp]: "lookup \<C> p = Some Return\<^sub>b \<Longrightarrow> 
     \<C> \<tturnstile> S\<^sub>b \<V> ((\<Delta>, Suc p) # s) \<leadsto>\<^sub>b S\<^sub>b \<V> s"
 | ev\<^sub>b_jump [simp]: "lookup \<C> p = Some Jump\<^sub>b \<Longrightarrow> 
