09HeapMemory/HeapConversion.thy
@@ -173,7 +173,7 @@ next
   moreover then obtain v\<^sub>h \<V>\<^sub>h where "\<V>\<^sub>h' = v\<^sub>h # \<V>\<^sub>h \<and> v\<^sub>b = unheap_closure h v\<^sub>h \<and> 
     \<V>\<^sub>b = map (unheap_closure h) \<V>\<^sub>h" by fastforce
   moreover from ev\<^sub>b_pushenv have "\<C> \<tturnstile> S\<^sub>h h (v\<^sub>h # \<V>\<^sub>h) ((\<Delta>\<^sub>h, Suc p) # s\<^sub>h) \<leadsto>\<^sub>h 
-    S\<^sub>h h \<V>\<^sub>h ((cons_fst v\<^sub>h \<Delta>\<^sub>h, p) # s\<^sub>h)" by simp
+    S\<^sub>h h \<V>\<^sub>h ((snoc_fst v\<^sub>h \<Delta>\<^sub>h, p) # s\<^sub>h)" by simp
   ultimately show ?case by fastforce
 next
   case (ev\<^sub>b_return \<C> p \<V>\<^sub>b \<Delta>\<^sub>b s\<^sub>b)
